Wrote up closure conversion

05Closure/ClosureConversion.thy
@@ -2,445 +2,424 @@ theory ClosureConversion
   imports Closure "../04Stack/Stack" "../03Debruijn/Multisubst"
 begin
 
+subsection \<open>Closure conversion\<close>
+
+text \<open>The basic relationship between closure-values and expressions is simple: the only complicated 
+case is closures proper, and by substituting in the entire environment at once using the multisubst 
+method we have already helpfully defined, we get an equivalent expression. Once again, however, any 
+number of closures could declose to a single expression, so we are forced to run our conversions 
+backwards.\<close>
+
 primrec declosure :: "closure\<^sub>c \<Rightarrow> expr\<^sub>d" where
-  "declosure (Const\<^sub>c k) = Const\<^sub>d k"
-| "declosure (Lam\<^sub>c t cs e) = multisubst (map declosure cs) (Lam\<^sub>d t e)"
+  "declosure (Const\<^sub>c n) = Const\<^sub>d n"
+| "declosure (Lam\<^sub>c t \<Delta> e) = multisubst (map declosure \<Delta>) (Lam\<^sub>d t e)"
 
-fun declosure_stack :: "frame\<^sub>c list \<Rightarrow> frame\<^sub>k list" where
-  "declosure_stack [] = []"
-| "declosure_stack (FApp1\<^sub>c cs e # s) = FApp1\<^sub>k (multisubst (map declosure cs) e) # declosure_stack s"
-| "declosure_stack (FApp2\<^sub>c c # s) = FApp2\<^sub>k (declosure c) # declosure_stack s"
-| "declosure_stack (FReturn\<^sub>c cs # s) = FReturn\<^sub>k # declosure_stack s"
-
-primrec destate\<^sub>c :: "state\<^sub>c \<Rightarrow> state\<^sub>k" where
-  "destate\<^sub>c (SE\<^sub>c s cs e) = S\<^sub>k False (declosure_stack s) (multisubst (map declosure cs) e)"
-| "destate\<^sub>c (SC\<^sub>c s c) = S\<^sub>k True (declosure_stack s) (declosure c)"
-
-lemma [simp]: "value\<^sub>d (declosure c)"
+lemma declosure_always_value [simp]: "value\<^sub>d (declosure c)"
 proof (induction c)
-  case (Lam\<^sub>c t cs e)
-  thus ?case by (induction cs arbitrary: e) simp_all
+  case (Lam\<^sub>c t \<Delta> e)
+  thus ?case by (induction \<Delta> arbitrary: e) simp_all
 qed simp_all
 
-lemma [simp]: "c :\<^sub>c\<^sub>l t \<Longrightarrow> [] \<turnstile>\<^sub>d declosure c : t"
-  and [simp]: "cs :\<^sub>c\<^sub>l\<^sub>s ts \<Longrightarrow> tc_expr_context ts (map declosure cs)" 
-proof (induction c t and cs ts rule: typing_closure\<^sub>c_typing_environment\<^sub>c.inducts)
-  case (tc\<^sub>c_lam cs ts t\<^sub>1 e t\<^sub>2)
-  then obtain e' where "multisubst (map declosure cs) (Lam\<^sub>d t\<^sub>1 e) = Lam\<^sub>d t\<^sub>1 e' \<and> ([t\<^sub>1] \<turnstile>\<^sub>d e' : t\<^sub>2) \<and> 
-    (\<forall>e\<^sub>2. ([] \<turnstile>\<^sub>d e\<^sub>2 : t\<^sub>1) \<longrightarrow> multisubst (map declosure cs) (subst\<^sub>d 0 e\<^sub>2 e) = subst\<^sub>d 0 e\<^sub>2 e')" 
+lemma tc_declosure [simp]: "c :\<^sub>c\<^sub>l t \<Longrightarrow> [] \<turnstile>\<^sub>d declosure c : t"
+  and tc_declosure_env [simp]: "\<Delta> :\<^sub>c\<^sub>l\<^sub>s \<Gamma> \<Longrightarrow> tc_expr_context \<Gamma> (map declosure \<Delta>)" 
+proof (induction c t and \<Delta> \<Gamma> rule: typing_closure\<^sub>c_typing_environment\<^sub>c.inducts)
+  case (tc\<^sub>c_lam \<Delta> \<Gamma> t\<^sub>1 e t\<^sub>2)
+  then obtain e' where "multisubst (map declosure \<Delta>) (Lam\<^sub>d t\<^sub>1 e) = Lam\<^sub>d t\<^sub>1 e' \<and> ([t\<^sub>1] \<turnstile>\<^sub>d e' : t\<^sub>2) \<and> 
+    (\<forall>e\<^sub>2. ([] \<turnstile>\<^sub>d e\<^sub>2 : t\<^sub>1) \<longrightarrow> multisubst (map declosure \<Delta>) (subst\<^sub>d 0 e\<^sub>2 e) = subst\<^sub>d 0 e\<^sub>2 e')" 
       by fastforce
   thus ?case by simp
 qed simp_all
 
-lemma [simp]: "s :\<^sub>c t' \<rightarrow> t \<Longrightarrow> declosure_stack s :\<^sub>k t' \<rightarrow> t"
-proof (induction s t' t rule: typing_stack\<^sub>c.induct)
-  case (tcc_scons_app1 cs ts e t\<^sub>1 s t\<^sub>2 t)
-  hence "tc_expr_context ts (map declosure cs)" by simp
-  moreover from tcc_scons_app1 have "ts \<turnstile>\<^sub>d e : t\<^sub>1" by simp
-  ultimately have "[] \<turnstile>\<^sub>d multisubst (map declosure cs) e : t\<^sub>1" by simp
-  with tcc_scons_app1 show ?case by simp
-next
-  case (tcc_scons_app2 c t\<^sub>1 t\<^sub>2 s t)
-  hence "[] \<turnstile>\<^sub>d declosure c : Arrow t\<^sub>1 t\<^sub>2" by simp
-  moreover from tcc_scons_app2 have "declosure_stack s :\<^sub>k t\<^sub>2 \<rightarrow> t" by simp
-  ultimately show ?case by simp
-qed simp_all
-  
-theorem typesafec [simp]: "\<Sigma> :\<^sub>c t \<Longrightarrow> destate\<^sub>c \<Sigma> :\<^sub>k t"
-proof (induction \<Sigma> t rule: typecheck_state\<^sub>c.induct)
-  case (tcc_state_ev s t' t cs ts e)
-  hence "tc_expr_context ts (map declosure cs)" by simp
-  moreover from tcc_state_ev have "ts \<turnstile>\<^sub>d e : t'" by simp
-  ultimately have "[] \<turnstile>\<^sub>d multisubst (map declosure cs) e : t'" by simp
-  moreover from tcc_state_ev have "declosure_stack s :\<^sub>k t' \<rightarrow> t" by simp
-  ultimately show ?case by simp
-next
-  case (tcc_state_ret s t' t c)
-  hence "declosure_stack s :\<^sub>k t' \<rightarrow> t" by simp
-  moreover from tcc_state_ret have "[] \<turnstile>\<^sub>d declosure c : t'" by simp
-  ultimately show ?case by simp
-qed
-
 lemma multisubst_closure [simp]: "c :\<^sub>c\<^sub>l t \<Longrightarrow> multisubst es (declosure c) = declosure c"
-  and [simp]: "cs :\<^sub>c\<^sub>l\<^sub>s ts \<Longrightarrow> v \<in> set (map declosure cs) \<Longrightarrow> multisubst es v = v"
-proof (induction c t and cs ts rule: typing_closure\<^sub>c_typing_environment\<^sub>c.inducts)
-  case (tc\<^sub>c_lam cs ts t\<^sub>1 e t\<^sub>2)
-  moreover hence "tc_expr_context ts (map declosure cs)" by simp
-  ultimately obtain e' where E: "multisubst (map declosure cs) (Lam\<^sub>d t\<^sub>1 e) = Lam\<^sub>d t\<^sub>1 e' \<and> 
+  and multisubst_env [simp]: "\<Delta> :\<^sub>c\<^sub>l\<^sub>s \<Gamma> \<Longrightarrow> v \<in> set (map declosure \<Delta>) \<Longrightarrow> multisubst es v = v"
+proof (induction c t and \<Delta> \<Gamma> rule: typing_closure\<^sub>c_typing_environment\<^sub>c.inducts)
+  case (tc\<^sub>c_lam \<Delta> \<Gamma> t\<^sub>1 e t\<^sub>2)
+  moreover hence "tc_expr_context \<Gamma> (map declosure \<Delta>)" by simp
+  ultimately obtain e' where E: "multisubst (map declosure \<Delta>) (Lam\<^sub>d t\<^sub>1 e) = Lam\<^sub>d t\<^sub>1 e' \<and> 
     ([t\<^sub>1] \<turnstile>\<^sub>d e' : t\<^sub>2) \<and> (\<forall>e\<^sub>2. ([] \<turnstile>\<^sub>d e\<^sub>2 : t\<^sub>1) \<longrightarrow> 
-      multisubst (map declosure cs) (subst\<^sub>d 0 e\<^sub>2 e) = subst\<^sub>d 0 e\<^sub>2 e')" by fastforce
+      multisubst (map declosure \<Delta>) (subst\<^sub>d 0 e\<^sub>2 e) = subst\<^sub>d 0 e\<^sub>2 e')" by fastforce
   hence "[] \<turnstile>\<^sub>d Lam\<^sub>d t\<^sub>1 e' : Arrow t\<^sub>1 t\<^sub>2" by simp
   hence "multisubst es (Lam\<^sub>d t\<^sub>1 e') = Lam\<^sub>d t\<^sub>1 e'" by simp
   with E show ?case by simp
 qed auto
 
-lemma [simp]: "c :\<^sub>c\<^sub>l t \<Longrightarrow> subst\<^sub>d 0 e' (declosure c) = declosure c"
-proof -
-  assume "c :\<^sub>c\<^sub>l t"
-  hence "multisubst [e'] (declosure c) = declosure c" by (metis multisubst_closure)
-  thus ?thesis by simp
+text \<open>The stack conversion is an easy extension. We throw away the extra environment on \<open>FReturn\<^sub>c\<close> 
+frames.\<close>
+
+fun declosure_stack :: "frame\<^sub>c list \<Rightarrow> frame\<^sub>k list" where
+  "declosure_stack [] = []"
+| "declosure_stack (FApp1\<^sub>c \<Delta> e # s\<^sub>c) = FApp1\<^sub>k (multisubst (map declosure \<Delta>) e) # declosure_stack s\<^sub>c"
+| "declosure_stack (FApp2\<^sub>c c # s\<^sub>c) = FApp2\<^sub>k (declosure c) # declosure_stack s\<^sub>c"
+| "declosure_stack (FReturn\<^sub>c \<Delta> # s\<^sub>c) = FReturn\<^sub>k # declosure_stack s\<^sub>c"
+
+lemma tc_declosure_stack [simp]: "s\<^sub>c :\<^sub>c t' \<rightarrow> t \<Longrightarrow> declosure_stack s\<^sub>c :\<^sub>k t' \<rightarrow> t"
+proof (induction s\<^sub>c t' t rule: typing_stack\<^sub>c.induct)
+  case (tcc_scons_app1 \<Delta> \<Gamma> e t\<^sub>1 s\<^sub>c t\<^sub>2 t)
+  hence "tc_expr_context \<Gamma> (map declosure \<Delta>)" by simp
+  moreover from tcc_scons_app1 have "\<Gamma> \<turnstile>\<^sub>d e : t\<^sub>1" by simp
+  ultimately have "[] \<turnstile>\<^sub>d multisubst (map declosure \<Delta>) e : t\<^sub>1" by simp
+  with tcc_scons_app1 show ?case by simp
+next
+  case (tcc_scons_app2 c t\<^sub>1 t\<^sub>2 s\<^sub>c t)
+  hence "[] \<turnstile>\<^sub>d declosure c : Arrow t\<^sub>1 t\<^sub>2" by simp
+  moreover from tcc_scons_app2 have "declosure_stack s\<^sub>c :\<^sub>k t\<^sub>2 \<rightarrow> t" by simp
+  ultimately show ?case by simp
+qed simp_all
+
+text \<open>The state level conversion follows, as does type safety and completeness. Completeness is 
+unfortunately complicated by the fact that _almost_ every closure evaluation step has an equivalent
+stack evaluation step; but looking up a variable takes a step in this stage, and didn't in the 
+previous (all variables were substituted away at the moment of function application), so we must 
+again use \<open>iter\<close>.\<close>
+
+primrec declosure_state :: "state\<^sub>c \<Rightarrow> state\<^sub>k" where
+  "declosure_state (SE\<^sub>c s\<^sub>c \<Delta> e) = S\<^sub>k False (declosure_stack s\<^sub>c) (multisubst (map declosure \<Delta>) e)"
+| "declosure_state (SC\<^sub>c s\<^sub>c c) = S\<^sub>k True (declosure_stack s\<^sub>c) (declosure c)"
+  
+theorem typesafe\<^sub>c [simp]: "\<Sigma>\<^sub>c :\<^sub>c t \<Longrightarrow> declosure_state \<Sigma>\<^sub>c :\<^sub>k t"
+proof (induction \<Sigma>\<^sub>c t rule: typecheck_state\<^sub>c.induct)
+  case (tcc_state_ev s\<^sub>c t' t \<Delta>\<^sub>c \<Gamma> e)
+  hence "tc_expr_context \<Gamma> (map declosure \<Delta>\<^sub>c)" by simp
+  moreover from tcc_state_ev have "\<Gamma> \<turnstile>\<^sub>d e : t'" by simp
+  ultimately have "[] \<turnstile>\<^sub>d multisubst (map declosure \<Delta>\<^sub>c) e : t'" by simp
+  moreover from tcc_state_ev have "declosure_stack s\<^sub>c :\<^sub>k t' \<rightarrow> t" by simp
+  ultimately show ?case by simp
+next
+  case (tcc_state_ret s\<^sub>c t' t c)
+  hence "declosure_stack s\<^sub>c :\<^sub>k t' \<rightarrow> t" by simp
+  moreover from tcc_state_ret have "[] \<turnstile>\<^sub>d declosure c : t'" by simp
+  ultimately show ?case by simp
 qed
 
-theorem correctc: "\<Sigma> \<leadsto>\<^sub>c \<Sigma>' \<Longrightarrow> \<Sigma> :\<^sub>c t \<Longrightarrow> iter (\<leadsto>\<^sub>k) (destate\<^sub>c \<Sigma>) (destate\<^sub>c \<Sigma>')"
-proof (induction \<Sigma> \<Sigma>' rule: eval\<^sub>c.induct)
-  case (ev\<^sub>c_var cs x c s)
-  then obtain t' ts where "(s :\<^sub>c t' \<rightarrow> t) \<and> (cs :\<^sub>c\<^sub>l\<^sub>s ts) \<and> lookup ts x = Some t'" by fastforce
-  hence "\<And>v es. v \<in> set (map declosure cs) \<Longrightarrow> multisubst es v = v" by auto
-  moreover from ev\<^sub>c_var have "lookup (map declosure cs) x = Some (declosure c)" by simp
-  ultimately have "multisubst (map declosure cs) (Var\<^sub>d x) = declosure c" by (metis multisubst_var)
+theorem completeness\<^sub>c: "\<Sigma>\<^sub>c \<leadsto>\<^sub>c \<Sigma>\<^sub>c' \<Longrightarrow> \<Sigma>\<^sub>c :\<^sub>c t \<Longrightarrow> 
+  iter (\<leadsto>\<^sub>k) (declosure_state \<Sigma>\<^sub>c) (declosure_state \<Sigma>\<^sub>c')"
+proof (induction \<Sigma>\<^sub>c \<Sigma>\<^sub>c' rule: eval\<^sub>c.induct)
+  case (ev\<^sub>c_var \<Delta> x c s\<^sub>c)
+  then obtain t' \<Gamma> where "(s\<^sub>c :\<^sub>c t' \<rightarrow> t) \<and> (\<Delta> :\<^sub>c\<^sub>l\<^sub>s \<Gamma>) \<and> lookup \<Gamma> x = Some t'" by fastforce
+  hence "\<And>v es. v \<in> set (map declosure \<Delta>) \<Longrightarrow> multisubst es v = v" by auto
+  moreover from ev\<^sub>c_var have "lookup (map declosure \<Delta>) x = Some (declosure c)" by simp
+  ultimately have "multisubst (map declosure \<Delta>) (Var\<^sub>d x) = declosure c" by (metis multisubst_var)
   thus ?case by simp
 next
-  case (ev\<^sub>c_lam s cs t e)
-  obtain e' where "multisubst (map declosure cs) (Lam\<^sub>d t e) = Lam\<^sub>d t e'" by fastforce
-  hence "S\<^sub>k False (declosure_stack s) (multisubst (map declosure cs) (Lam\<^sub>d t e)) \<leadsto>\<^sub>k
-    S\<^sub>k True (declosure_stack s) (multisubst (map declosure cs) (Lam\<^sub>d t e))" by simp
-  hence "iter (\<leadsto>\<^sub>k) (S\<^sub>k False (declosure_stack s) (multisubst (map declosure cs) (Lam\<^sub>d t e)))
-    (S\<^sub>k True (declosure_stack s) (multisubst (map declosure cs) (Lam\<^sub>d t e)))" 
+  case (ev\<^sub>c_lam s\<^sub>c \<Delta> t e)
+  obtain e' where "multisubst (map declosure \<Delta>) (Lam\<^sub>d t e) = Lam\<^sub>d t e'" by fastforce
+  hence "S\<^sub>k False (declosure_stack s\<^sub>c) (multisubst (map declosure \<Delta>) (Lam\<^sub>d t e)) \<leadsto>\<^sub>k
+    S\<^sub>k True (declosure_stack s\<^sub>c) (multisubst (map declosure \<Delta>) (Lam\<^sub>d t e))" by simp
+  hence "iter (\<leadsto>\<^sub>k) (S\<^sub>k False (declosure_stack s\<^sub>c) (multisubst (map declosure \<Delta>) (Lam\<^sub>d t e)))
+    (S\<^sub>k True (declosure_stack s\<^sub>c) (multisubst (map declosure \<Delta>) (Lam\<^sub>d t e)))" 
       by (metis iter_step iter_refl)
   thus ?case by simp
 next
-  case (ev\<^sub>c_app s cs e\<^sub>1 e\<^sub>2)
-  have "S\<^sub>k False (declosure_stack s) (App\<^sub>d (multisubst (map declosure cs) e\<^sub>1) 
-    (multisubst (map declosure cs) e\<^sub>2)) \<leadsto>\<^sub>k 
-      S\<^sub>k False (FApp1\<^sub>k (multisubst (map declosure cs) e\<^sub>2) # declosure_stack s) 
-        (multisubst (map declosure cs) e\<^sub>1)" by simp
-  hence "iter (\<leadsto>\<^sub>k) (S\<^sub>k False (declosure_stack s) (App\<^sub>d (multisubst (map declosure cs) e\<^sub>1) 
-    (multisubst (map declosure cs) e\<^sub>2))) 
-      (S\<^sub>k False (FApp1\<^sub>k (multisubst (map declosure cs) e\<^sub>2) # declosure_stack s) 
-        (multisubst (map declosure cs) e\<^sub>1))" by (metis iter_step iter_refl)
+  case (ev\<^sub>c_app s\<^sub>c \<Delta> e\<^sub>1 e\<^sub>2)
+  have "S\<^sub>k False (declosure_stack s\<^sub>c) (App\<^sub>d (multisubst (map declosure \<Delta>) e\<^sub>1) 
+    (multisubst (map declosure \<Delta>) e\<^sub>2)) \<leadsto>\<^sub>k 
+      S\<^sub>k False (FApp1\<^sub>k (multisubst (map declosure \<Delta>) e\<^sub>2) # declosure_stack s\<^sub>c) 
+        (multisubst (map declosure \<Delta>) e\<^sub>1)" by simp
+  hence "iter (\<leadsto>\<^sub>k) (S\<^sub>k False (declosure_stack s\<^sub>c) (App\<^sub>d (multisubst (map declosure \<Delta>) e\<^sub>1) 
+    (multisubst (map declosure \<Delta>) e\<^sub>2))) 
+      (S\<^sub>k False (FApp1\<^sub>k (multisubst (map declosure \<Delta>) e\<^sub>2) # declosure_stack s\<^sub>c) 
+        (multisubst (map declosure \<Delta>) e\<^sub>1))" by (metis iter_step iter_refl)
   thus ?case by simp
 next
-  case (ret\<^sub>c_app1 cs e\<^sub>2 s c\<^sub>1)
-  have "S\<^sub>k True (FApp1\<^sub>k (multisubst (map declosure cs) e\<^sub>2) # declosure_stack s) (declosure c\<^sub>1) \<leadsto>\<^sub>k
-    S\<^sub>k False (FApp2\<^sub>k (declosure c\<^sub>1) # declosure_stack s) (multisubst (map declosure cs) e\<^sub>2)" by simp
-  hence "iter (\<leadsto>\<^sub>k) (S\<^sub>k True (FApp1\<^sub>k (multisubst (map declosure cs) e\<^sub>2) # declosure_stack s) 
+  case (ret\<^sub>c_app1 \<Delta> e\<^sub>2 s\<^sub>c c\<^sub>1)
+  have "S\<^sub>k True (FApp1\<^sub>k (multisubst (map declosure \<Delta>) e\<^sub>2) # declosure_stack s\<^sub>c) (declosure c\<^sub>1) \<leadsto>\<^sub>k
+    S\<^sub>k False (FApp2\<^sub>k (declosure c\<^sub>1) # declosure_stack s\<^sub>c) (multisubst (map declosure \<Delta>) e\<^sub>2)" by simp
+  hence "iter (\<leadsto>\<^sub>k) (S\<^sub>k True (FApp1\<^sub>k (multisubst (map declosure \<Delta>) e\<^sub>2) # declosure_stack s\<^sub>c) 
     (declosure c\<^sub>1)) 
-      (S\<^sub>k False (FApp2\<^sub>k (declosure c\<^sub>1) # declosure_stack s) (multisubst (map declosure cs) e\<^sub>2))" 
+      (S\<^sub>k False (FApp2\<^sub>k (declosure c\<^sub>1) # declosure_stack s\<^sub>c) (multisubst (map declosure \<Delta>) e\<^sub>2))" 
         by (metis iter_step iter_refl)
   thus ?case by simp
 next
-  case (ret\<^sub>c_app2 t\<^sub>1 cs e\<^sub>1 s c\<^sub>2)
-  then obtain ts t\<^sub>2 where T: "(cs :\<^sub>c\<^sub>l\<^sub>s ts) \<and> (insert_at 0 t\<^sub>1 ts \<turnstile>\<^sub>d e\<^sub>1 : t\<^sub>2) \<and> (s :\<^sub>c t\<^sub>2 \<rightarrow> t) \<and> 
+  case (ret\<^sub>c_app2 t\<^sub>1 \<Delta> e\<^sub>1 s\<^sub>c c\<^sub>2)
+  then obtain \<Gamma> t\<^sub>2 where T: "(\<Delta> :\<^sub>c\<^sub>l\<^sub>s \<Gamma>) \<and> (insert_at 0 t\<^sub>1 \<Gamma> \<turnstile>\<^sub>d e\<^sub>1 : t\<^sub>2) \<and> (s\<^sub>c :\<^sub>c t\<^sub>2 \<rightarrow> t) \<and> 
     (c\<^sub>2 :\<^sub>c\<^sub>l t\<^sub>1)" by fastforce
-  hence "tc_expr_context ts (map declosure cs) \<and> insert_at 0 t\<^sub>1 ts \<turnstile>\<^sub>d e\<^sub>1 : t\<^sub>2" by simp
-  then obtain e' where "multisubst (map declosure cs) (Lam\<^sub>d t\<^sub>1 e\<^sub>1) = Lam\<^sub>d t\<^sub>1 e' \<and> ([t\<^sub>1] \<turnstile>\<^sub>d e' : t\<^sub>2) \<and>
-    (\<forall>e\<^sub>2. ([] \<turnstile>\<^sub>d e\<^sub>2 : t\<^sub>1) \<longrightarrow> multisubst (map declosure cs) (subst\<^sub>d 0 e\<^sub>2 e\<^sub>1) = subst\<^sub>d 0 e\<^sub>2 e')" 
+  hence "tc_expr_context \<Gamma> (map declosure \<Delta>) \<and> insert_at 0 t\<^sub>1 \<Gamma> \<turnstile>\<^sub>d e\<^sub>1 : t\<^sub>2" by simp
+  then obtain e' where "multisubst (map declosure \<Delta>) (Lam\<^sub>d t\<^sub>1 e\<^sub>1) = Lam\<^sub>d t\<^sub>1 e' \<and> ([t\<^sub>1] \<turnstile>\<^sub>d e' : t\<^sub>2) \<and>
+    (\<forall>e\<^sub>2. ([] \<turnstile>\<^sub>d e\<^sub>2 : t\<^sub>1) \<longrightarrow> multisubst (map declosure \<Delta>) (subst\<^sub>d 0 e\<^sub>2 e\<^sub>1) = subst\<^sub>d 0 e\<^sub>2 e')" 
       by fastforce
-  with T have "S\<^sub>k True (FApp2\<^sub>k (multisubst (map declosure cs) (Lam\<^sub>d t\<^sub>1 e\<^sub>1)) # declosure_stack s) 
-    (declosure c\<^sub>2) \<leadsto>\<^sub>k (S\<^sub>k False (FReturn\<^sub>k # declosure_stack s) 
-      (multisubst (map declosure cs) (subst\<^sub>d 0 (declosure c\<^sub>2) e\<^sub>1)))" 
+  with T have "S\<^sub>k True (FApp2\<^sub>k (multisubst (map declosure \<Delta>) (Lam\<^sub>d t\<^sub>1 e\<^sub>1)) # declosure_stack s\<^sub>c) 
+    (declosure c\<^sub>2) \<leadsto>\<^sub>k (S\<^sub>k False (FReturn\<^sub>k # declosure_stack s\<^sub>c) 
+      (multisubst (map declosure \<Delta>) (subst\<^sub>d 0 (declosure c\<^sub>2) e\<^sub>1)))" 
     by simp
-  hence "iter (\<leadsto>\<^sub>k) (S\<^sub>k True (FApp2\<^sub>k (multisubst (map declosure cs) (Lam\<^sub>d t\<^sub>1 e\<^sub>1)) # declosure_stack s) 
+  hence "iter (\<leadsto>\<^sub>k) (S\<^sub>k True (FApp2\<^sub>k (multisubst (map declosure \<Delta>) (Lam\<^sub>d t\<^sub>1 e\<^sub>1)) # declosure_stack s\<^sub>c) 
     (declosure c\<^sub>2)) 
-      (S\<^sub>k False (FReturn\<^sub>k # declosure_stack s) 
-        (multisubst (map declosure cs) (subst\<^sub>d 0 (declosure c\<^sub>2) e\<^sub>1)))" 
+      (S\<^sub>k False (FReturn\<^sub>k # declosure_stack s\<^sub>c) 
+        (multisubst (map declosure \<Delta>) (subst\<^sub>d 0 (declosure c\<^sub>2) e\<^sub>1)))" 
     by (metis iter_step iter_refl)
   thus ?case by simp
 next
-  case (ret\<^sub>c_ret cs s c)
-  have "S\<^sub>k True (FReturn\<^sub>k # declosure_stack s) (declosure c) \<leadsto>\<^sub>k 
-    S\<^sub>k True (declosure_stack s) (declosure c)" by simp
-  hence "iter (\<leadsto>\<^sub>k) (S\<^sub>k True (FReturn\<^sub>k # declosure_stack s) (declosure c)) 
-    (S\<^sub>k True (declosure_stack s) (declosure c))" by (metis iter_step iter_refl)
+  case (ret\<^sub>c_ret \<Delta> s\<^sub>c c)
+  have "S\<^sub>k True (FReturn\<^sub>k # declosure_stack s\<^sub>c) (declosure c) \<leadsto>\<^sub>k 
+    S\<^sub>k True (declosure_stack s\<^sub>c) (declosure c)" by simp
+  hence "iter (\<leadsto>\<^sub>k) (S\<^sub>k True (FReturn\<^sub>k # declosure_stack s\<^sub>c) (declosure c)) 
+    (S\<^sub>k True (declosure_stack s\<^sub>c) (declosure c))" by (metis iter_step iter_refl)
   thus ?case by simp
 qed simp_all
 
-lemma [simp]: "[] = declosure_stack s \<Longrightarrow> s = []"
-  by (induction s rule: declosure_stack.induct) simp_all
+text \<open>Once again, correctness is more difficult, and requires reconstruction lemmas. Unlike last 
+time, where a single (albeit complicated) lemma sufficed, closure conversion involves three separate 
+levels of conversion, and a correspondingly larger number of lemmas. Fortunately, since there is a 
+closer relation between stacks and states, most of them are much simpler to state and prove.\<close>
 
-lemma [simp]: "FApp1\<^sub>k e # s = declosure_stack s\<^sub>c \<Longrightarrow> \<exists>cs e' s\<^sub>c'. s\<^sub>c = FApp1\<^sub>c cs e' # s\<^sub>c' \<and> 
-    e = multisubst (map declosure cs) e' \<and> s = declosure_stack s\<^sub>c'"
-  by (induction s\<^sub>c rule: declosure_stack.induct) simp_all
-
-lemma [simp]: "FApp2\<^sub>k e # s = declosure_stack s\<^sub>c \<Longrightarrow> 
-    \<exists>c s\<^sub>c'. s\<^sub>c = FApp2\<^sub>c c # s\<^sub>c' \<and> e = declosure c \<and> s = declosure_stack s\<^sub>c'"
-  by (induction s\<^sub>c rule: declosure_stack.induct) simp_all
-
-lemma [simp]: "FReturn\<^sub>k # s = declosure_stack s\<^sub>c \<Longrightarrow> \<exists>cs s\<^sub>c'. s\<^sub>c = FReturn\<^sub>c cs # s\<^sub>c'"
-  by (induction s\<^sub>c rule: declosure_stack.induct) simp_all
-
-lemma [dest]: "S\<^sub>k b s e = destate\<^sub>c \<Sigma> \<Longrightarrow> 
-  \<exists>s'. s = declosure_stack s' \<and> 
-    ((\<exists>cs e'. \<not> b \<and> \<Sigma> = SE\<^sub>c s' cs e' \<and> e = multisubst (map declosure cs) e') \<or> 
-      (\<exists>c. b \<and> \<Sigma> = SC\<^sub>c s' c \<and> e = declosure c))"
-  by (induction \<Sigma>) simp_all
-
-lemma [dest]: "App\<^sub>d e\<^sub>1 e\<^sub>2 = multisubst (map declosure cs) (Lam\<^sub>d t e) \<Longrightarrow> False"
-proof -
-  assume "App\<^sub>d e\<^sub>1 e\<^sub>2 = multisubst (map declosure cs) (Lam\<^sub>d t e)"
-  moreover obtain e' where "multisubst (map declosure cs) (Lam\<^sub>d t e) = Lam\<^sub>d t e'" by fastforce
-  ultimately show ?thesis by simp
-qed
-
-lemma lam_to_declosure [simp]: "Lam\<^sub>d t\<^sub>1 e = declosure c \<Longrightarrow> c :\<^sub>c\<^sub>l Arrow t' t\<^sub>2 \<Longrightarrow>
-  \<exists>cs e'. c = Lam\<^sub>c t\<^sub>1 cs e' \<and> multisubst (map declosure cs) (Lam\<^sub>d t\<^sub>1 e') = Lam\<^sub>d t\<^sub>1 e \<and> 
+lemma declose_to_lam [dest]: "Lam\<^sub>d t\<^sub>1 e = declosure c \<Longrightarrow> c :\<^sub>c\<^sub>l Arrow t' t\<^sub>2 \<Longrightarrow>
+  \<exists>\<Delta> e'. c = Lam\<^sub>c t\<^sub>1 \<Delta> e' \<and> multisubst (map declosure \<Delta>) (Lam\<^sub>d t\<^sub>1 e') = Lam\<^sub>d t\<^sub>1 e \<and> 
     ([t\<^sub>1] \<turnstile>\<^sub>d e : t\<^sub>2) \<and> t' = t\<^sub>1 \<and>
-    (\<forall>e\<^sub>2. ([] \<turnstile>\<^sub>d e\<^sub>2 : t\<^sub>1) \<longrightarrow> multisubst (map declosure cs) (subst\<^sub>d 0 e\<^sub>2 e') = subst\<^sub>d 0 e\<^sub>2 e)"
+    (\<forall>e\<^sub>2. ([] \<turnstile>\<^sub>d e\<^sub>2 : t\<^sub>1) \<longrightarrow> multisubst (map declosure \<Delta>) (subst\<^sub>d 0 e\<^sub>2 e') = subst\<^sub>d 0 e\<^sub>2 e)"
 proof (induction c)
-  case (Lam\<^sub>c tt cs e')
-  moreover then obtain ts where T: "(cs :\<^sub>c\<^sub>l\<^sub>s ts) \<and> (insert_at 0 t' ts \<turnstile>\<^sub>d e' : t\<^sub>2) \<and> tt = t'" 
+  case (Lam\<^sub>c tt \<Delta> e')
+  moreover then obtain \<Gamma> where T: "(\<Delta> :\<^sub>c\<^sub>l\<^sub>s \<Gamma>) \<and> (insert_at 0 t' \<Gamma> \<turnstile>\<^sub>d e' : t\<^sub>2) \<and> tt = t'" 
     by fastforce
-  moreover hence "tc_expr_context ts (map declosure cs)" by simp
-  ultimately obtain e'' where "multisubst (map declosure cs) (Lam\<^sub>d t' e') = Lam\<^sub>d t' e'' \<and> 
+  moreover hence "tc_expr_context \<Gamma> (map declosure \<Delta>)" by simp
+  ultimately obtain e'' where "multisubst (map declosure \<Delta>) (Lam\<^sub>d t' e') = Lam\<^sub>d t' e'' \<and> 
     ([t'] \<turnstile>\<^sub>d e'' : t\<^sub>2) \<and>
-    (\<forall>e\<^sub>2. ([] \<turnstile>\<^sub>d e\<^sub>2 : t') \<longrightarrow> multisubst (map declosure cs) (subst\<^sub>d 0 e\<^sub>2 e') = subst\<^sub>d 0 e\<^sub>2 e'')"
+    (\<forall>e\<^sub>2. ([] \<turnstile>\<^sub>d e\<^sub>2 : t') \<longrightarrow> multisubst (map declosure \<Delta>) (subst\<^sub>d 0 e\<^sub>2 e') = subst\<^sub>d 0 e\<^sub>2 e'')"
       by fastforce
   with Lam\<^sub>c T show ?case by simp
 qed simp_all
 
-lemma [dest]: "App\<^sub>d e\<^sub>1 e\<^sub>2 = declosure c \<Longrightarrow> False"
+lemma declose_to_app [dest]: "App\<^sub>d e\<^sub>1 e\<^sub>2 = declosure c \<Longrightarrow> False"
   by (induction c) auto
 
-lemma [dest]: "App\<^sub>d e\<^sub>1 e\<^sub>2 = multisubst (map declosure cs) (declosure c) \<Longrightarrow> False"
+lemma declose_to_nil [dest]: "[] = declosure_stack s\<^sub>c \<Longrightarrow> s\<^sub>c = []"
+  by (induction s\<^sub>c rule: declosure_stack.induct) simp_all
+
+lemma declose_to_fapp1 [dest]: "FApp1\<^sub>k e # s\<^sub>k = declosure_stack s\<^sub>c \<Longrightarrow> 
+  \<exists>\<Delta> e' s\<^sub>c'. s\<^sub>c = FApp1\<^sub>c \<Delta> e' # s\<^sub>c' \<and> e = multisubst (map declosure \<Delta>) e' \<and> 
+    s\<^sub>k = declosure_stack s\<^sub>c'"
+  by (induction s\<^sub>c rule: declosure_stack.induct) simp_all
+
+lemma declose_to_fapp2 [dest]: "FApp2\<^sub>k e # s\<^sub>k = declosure_stack s\<^sub>c \<Longrightarrow> 
+    \<exists>c s\<^sub>c'. s\<^sub>c = FApp2\<^sub>c c # s\<^sub>c' \<and> e = declosure c \<and> s\<^sub>k = declosure_stack s\<^sub>c'"
+  by (induction s\<^sub>c rule: declosure_stack.induct) simp_all
+
+lemma declose_to_freturn [dest]: "FReturn\<^sub>k # s\<^sub>k = declosure_stack s\<^sub>c \<Longrightarrow> 
+    \<exists>\<Delta> s\<^sub>c'. s\<^sub>c = FReturn\<^sub>c \<Delta> # s\<^sub>c' \<and> s\<^sub>k = declosure_stack s\<^sub>c'"
+  by (induction s\<^sub>c rule: declosure_stack.induct) simp_all
+
+lemma declose_to_state [dest]: "S\<^sub>k b s\<^sub>k e = declosure_state \<Sigma>\<^sub>c \<Longrightarrow> 
+  \<exists>s\<^sub>c. s\<^sub>k = declosure_stack s\<^sub>c \<and> 
+    ((\<exists>\<Delta> e'. \<not> b \<and> \<Sigma>\<^sub>c = SE\<^sub>c s\<^sub>c \<Delta> e' \<and> e = multisubst (map declosure \<Delta>) e') \<or> 
+    (\<exists>c. b \<and> \<Sigma>\<^sub>c = SC\<^sub>c s\<^sub>c c \<and> e = declosure c))"
+  by (induction \<Sigma>\<^sub>c) simp_all
+
+lemma multisubst_closure_to_app [dest]: "App\<^sub>d e\<^sub>1 e\<^sub>2 = multisubst (map declosure \<Delta>) (declosure c) \<Longrightarrow>
+  False"
 proof (induction c)
-  case (Lam\<^sub>c t cs' e)
-  moreover obtain e' where "multisubst (map declosure cs') (Lam\<^sub>d t e) = Lam\<^sub>d t e'" by fastforce
+  case (Lam\<^sub>c t \<Delta>' e)
+  moreover obtain e' where "multisubst (map declosure \<Delta>') (Lam\<^sub>d t e) = Lam\<^sub>d t e'" by fastforce
   ultimately show ?case by auto
 qed simp_all 
 
-lemma [dest]: "App\<^sub>d e\<^sub>1 e\<^sub>2 = multisubst (map declosure cs) (Var\<^sub>d x) \<Longrightarrow> False"
-  by (induction cs x rule: lookup.induct) auto
+lemma multisusbt_var_to_app [dest]: "App\<^sub>d e\<^sub>1 e\<^sub>2 = multisubst (map declosure \<Delta>) (Var\<^sub>d x) \<Longrightarrow> False"
+  by (induction \<Delta> x rule: lookup.induct) auto
 
-lemma [simp]: "App\<^sub>d e\<^sub>1 e\<^sub>2 = multisubst (map declosure cs) e \<Longrightarrow> \<exists>e\<^sub>1' e\<^sub>2'. e = App\<^sub>d e\<^sub>1' e\<^sub>2' \<and>
-    e\<^sub>1 = multisubst (map declosure cs) e\<^sub>1' \<and> e\<^sub>2 = multisubst (map declosure cs) e\<^sub>2'"
+lemma multisusbt_to_app [dest]: "App\<^sub>d e\<^sub>1 e\<^sub>2 = multisubst (map declosure \<Delta>) e \<Longrightarrow> 
+  \<exists>e\<^sub>1' e\<^sub>2'. e = App\<^sub>d e\<^sub>1' e\<^sub>2' \<and> e\<^sub>1 = multisubst (map declosure \<Delta>) e\<^sub>1' \<and> 
+    e\<^sub>2 = multisubst (map declosure \<Delta>) e\<^sub>2'"
   by (induction e) auto
 
-lemma [dest]: "Const\<^sub>d k = multisubst es (declosure c) \<Longrightarrow> c = Const\<^sub>c k"
+lemma multisubst_closure_to_con [dest]: "Const\<^sub>d n = multisubst es (declosure c) \<Longrightarrow> c = Const\<^sub>c n"
 proof (induction c)
-  case (Lam\<^sub>c t cs e)
-  moreover obtain e' where "multisubst (map declosure cs) (Lam\<^sub>d t e) = Lam\<^sub>d t e'" by fastforce
+  case (Lam\<^sub>c t \<Delta> e)
+  moreover obtain e' where "multisubst (map declosure \<Delta>) (Lam\<^sub>d t e) = Lam\<^sub>d t e'" by fastforce
   moreover obtain e'' where "multisubst es (Lam\<^sub>d t e') = Lam\<^sub>d t e''" by fastforce
   ultimately show ?case by simp
 qed simp_all
 
-lemma [dest]: "Const\<^sub>d k = multisubst (map declosure cs) (Var\<^sub>d x) \<Longrightarrow> lookup cs x = Some (Const\<^sub>c k)"
-  by (induction cs x rule: lookup.induct) auto
+lemma multisubst_var_to_con [dest]: "Const\<^sub>d n = multisubst (map declosure \<Delta>) (Var\<^sub>d x) \<Longrightarrow> 
+    lookup \<Delta> x = Some (Const\<^sub>c n)"
+  by (induction \<Delta> x rule: lookup.induct) auto
 
-lemma [dest]: "Const\<^sub>d k = multisubst (map declosure cs) e \<Longrightarrow>
-    e = Const\<^sub>d k \<or> (\<exists>x. e = Var\<^sub>d x \<and> lookup cs x = Some (Const\<^sub>c k))"
+lemma multisubst_to_con [dest]: "Const\<^sub>d n = multisubst (map declosure \<Delta>) e \<Longrightarrow>
+  e = Const\<^sub>d n \<or> (\<exists>x. e = Var\<^sub>d x \<and> lookup \<Delta> x = Some (Const\<^sub>c n))"
 proof (induction e)
   case (Lam\<^sub>d t e)
-  moreover then obtain e' where "multisubst (map declosure cs) (Lam\<^sub>d t e) = Lam\<^sub>d t e'" by force
+  moreover then obtain e' where "multisubst (map declosure \<Delta>) (Lam\<^sub>d t e) = Lam\<^sub>d t e'" by force
   ultimately show ?case by simp
 qed auto
 
-lemma [simp]: "c :\<^sub>c\<^sub>l t \<Longrightarrow> incr\<^sub>d x (declosure c) = declosure c"
-  and [simp]: "cs :\<^sub>c\<^sub>l\<^sub>s ts \<Longrightarrow> ts \<turnstile>\<^sub>d e : tt \<Longrightarrow> 
-    incr\<^sub>d x (multisubst (map declosure cs) e) = multisubst (map declosure cs) e"
-proof (induction c t and cs ts arbitrary: and e tt 
+lemma incr_declosure [simp]: "c :\<^sub>c\<^sub>l t \<Longrightarrow> incr\<^sub>d x (declosure c) = declosure c"
+  and "\<Delta> :\<^sub>c\<^sub>l\<^sub>s \<Gamma> \<Longrightarrow> \<Gamma> \<turnstile>\<^sub>d e : tt \<Longrightarrow> 
+    incr\<^sub>d x (multisubst (map declosure \<Delta>) e) = multisubst (map declosure \<Delta>) e"
+proof (induction c t and \<Delta> \<Gamma> arbitrary: and e tt 
        rule: typing_closure\<^sub>c_typing_environment\<^sub>c.inducts)
-  case (tc\<^sub>c_lam cs ts t\<^sub>1 e t\<^sub>2)
-  moreover hence "ts \<turnstile>\<^sub>d Lam\<^sub>d t\<^sub>1 e : Arrow t\<^sub>1 t\<^sub>2" by simp
-  ultimately have "incr\<^sub>d x (multisubst (map declosure cs) (Lam\<^sub>d t\<^sub>1 e)) = 
-    multisubst (map declosure cs) (Lam\<^sub>d t\<^sub>1 e)" by blast
+  case (tc\<^sub>c_lam \<Delta> \<Gamma> t\<^sub>1 e t\<^sub>2)
+  moreover hence "\<Gamma> \<turnstile>\<^sub>d Lam\<^sub>d t\<^sub>1 e : Arrow t\<^sub>1 t\<^sub>2" by simp
+  ultimately have "incr\<^sub>d x (multisubst (map declosure \<Delta>) (Lam\<^sub>d t\<^sub>1 e)) = 
+    multisubst (map declosure \<Delta>) (Lam\<^sub>d t\<^sub>1 e)" by blast
   thus ?case by simp
 next
-  case (tc\<^sub>c_cons c t cs ts)
+  case (tc\<^sub>c_cons c t \<Delta> \<Gamma>)
   hence "[] \<turnstile>\<^sub>d declosure c : t" by simp
-  hence "ts \<turnstile>\<^sub>d declosure c : t" using tc_postpend by fastforce
-  moreover from tc\<^sub>c_cons have "insert_at 0 t ts \<turnstile>\<^sub>d e : tt" by (cases ts) simp_all
-  ultimately have "ts \<turnstile>\<^sub>d subst\<^sub>d 0 (declosure c) e : tt" by simp
+  hence "\<Gamma> \<turnstile>\<^sub>d declosure c : t" using tc_postpend by fastforce
+  moreover from tc\<^sub>c_cons have "insert_at 0 t \<Gamma> \<turnstile>\<^sub>d e : tt" by (cases \<Gamma>) simp_all
+  ultimately have "\<Gamma> \<turnstile>\<^sub>d subst\<^sub>d 0 (declosure c) e : tt" by simp
   with tc\<^sub>c_cons show ?case by simp
 qed simp_all
 
-lemma [simp]: "c :\<^sub>c\<^sub>l t \<Longrightarrow> True"
-  and [simp]: "cs :\<^sub>c\<^sub>l\<^sub>s ts \<Longrightarrow> insert_at 0 t\<^sub>1 ts \<turnstile>\<^sub>d e : t\<^sub>2 \<Longrightarrow> 
-  multisubst (map declosure cs') (multisubst (map declosure cs) (Lam\<^sub>d t\<^sub>1 e)) = 
-    multisubst (map declosure cs) (Lam\<^sub>d t\<^sub>1 e)"
-proof (induction c t and cs ts arbitrary: and e rule: typing_closure\<^sub>c_typing_environment\<^sub>c.inducts)
+lemma "c :\<^sub>c\<^sub>l t \<Longrightarrow> True"
+  and multisubst_lam_twice [simp]: "\<Delta> :\<^sub>c\<^sub>l\<^sub>s \<Gamma> \<Longrightarrow> insert_at 0 t\<^sub>1 \<Gamma> \<turnstile>\<^sub>d e : t\<^sub>2 \<Longrightarrow> 
+  multisubst (map declosure \<Delta>') (multisubst (map declosure \<Delta>) (Lam\<^sub>d t\<^sub>1 e)) = 
+    multisubst (map declosure \<Delta>) (Lam\<^sub>d t\<^sub>1 e)"
+proof (induction c t and \<Delta> \<Gamma> arbitrary: and e rule: typing_closure\<^sub>c_typing_environment\<^sub>c.inducts)
   case tc\<^sub>c_nil
-  thus ?case by (induction cs') simp_all
+  thus ?case by (induction \<Delta>') simp_all
 next
-  case (tc\<^sub>c_cons c t cs ts)
+  case (tc\<^sub>c_cons c t \<Delta> \<Gamma>)
   hence "[] \<turnstile>\<^sub>d declosure c : t" by simp
-  hence "insert_at 0 t\<^sub>1 ts \<turnstile>\<^sub>d declosure c : t" using tc_postpend by fastforce
-  with tc\<^sub>c_cons show ?case by (cases ts) simp_all
+  hence "insert_at 0 t\<^sub>1 \<Gamma> \<turnstile>\<^sub>d declosure c : t" using tc_postpend by fastforce
+  with tc\<^sub>c_cons show ?case by (cases \<Gamma>) simp_all
 qed simp_all
 
-lemma [dest]: "c :\<^sub>c\<^sub>l tt \<Longrightarrow> Lam\<^sub>d t e = multisubst (map declosure cs) (declosure c) \<Longrightarrow>
-  \<exists>cs' e'. c = Lam\<^sub>c t cs' e' \<and> 
-    multisubst (map declosure cs') (Lam\<^sub>d t e') = multisubst (map declosure cd) (declosure c)"
+lemma multisubst_closure_to_lam [dest]: "c :\<^sub>c\<^sub>l tt \<Longrightarrow> 
+  Lam\<^sub>d t e = multisubst (map declosure \<Delta>) (declosure c) \<Longrightarrow> \<exists>\<Delta>' e'. c = Lam\<^sub>c t \<Delta>' e' \<and> 
+    multisubst (map declosure \<Delta>') (Lam\<^sub>d t e') = multisubst (map declosure \<Delta>) (declosure c)"
 proof (induction c)
-  case (Lam\<^sub>c t\<^sub>1 cs' e')
-  then obtain t\<^sub>2 ts where T: "tt = Arrow t\<^sub>1 t\<^sub>2 \<and> (cs' :\<^sub>c\<^sub>l\<^sub>s ts) \<and> (insert_at 0 t\<^sub>1 ts \<turnstile>\<^sub>d e' : t\<^sub>2)" 
+  case (Lam\<^sub>c t\<^sub>1 \<Delta>' e')
+  then obtain t\<^sub>2 \<Gamma> where T: "tt = Arrow t\<^sub>1 t\<^sub>2 \<and> (\<Delta>' :\<^sub>c\<^sub>l\<^sub>s \<Gamma>) \<and> (insert_at 0 t\<^sub>1 \<Gamma> \<turnstile>\<^sub>d e' : t\<^sub>2)" 
     by fastforce
-  hence M: "multisubst (map declosure cs') (Lam\<^sub>d t\<^sub>1 e') = 
-      multisubst (map declosure cd) (multisubst (map declosure cs') (Lam\<^sub>d t\<^sub>1 e'))" by fastforce
-  obtain e2 where E: "multisubst (map declosure cs') (Lam\<^sub>d t\<^sub>1 e') = Lam\<^sub>d t\<^sub>1 e2" by fastforce
-  obtain e3 where "multisubst (map declosure cs) (Lam\<^sub>d t\<^sub>1 e2) = Lam\<^sub>d t\<^sub>1 e3" by fastforce
+  hence M: "multisubst (map declosure \<Delta>') (Lam\<^sub>d t\<^sub>1 e') = 
+      multisubst (map declosure \<Delta>) (multisubst (map declosure \<Delta>') (Lam\<^sub>d t\<^sub>1 e'))" by fastforce
+  obtain e2 where E: "multisubst (map declosure \<Delta>') (Lam\<^sub>d t\<^sub>1 e') = Lam\<^sub>d t\<^sub>1 e2" by fastforce
+  obtain e3 where "multisubst (map declosure \<Delta>) (Lam\<^sub>d t\<^sub>1 e2) = Lam\<^sub>d t\<^sub>1 e3" by fastforce
   with Lam\<^sub>c M E show ?case by simp
 qed simp_all
 
-lemma [dest]: "cs :\<^sub>c\<^sub>l\<^sub>s ts \<Longrightarrow> lookup ts x = Some tt \<Longrightarrow> 
-  Lam\<^sub>d t e = multisubst (map declosure cs) (Var\<^sub>d x) \<Longrightarrow> 
-    \<exists>cs' e'. lookup cs x = Some (Lam\<^sub>c t cs' e') \<and> 
-      multisubst (map declosure cs') (Lam\<^sub>d t e') = multisubst (map declosure cs) (Var\<^sub>d x)"
-  by (induction cs x arbitrary: ts rule: lookup.induct) fastforce+
+lemma multisubst_var_to_lam [dest]: "\<Delta> :\<^sub>c\<^sub>l\<^sub>s \<Gamma> \<Longrightarrow> lookup \<Gamma> x = Some tt \<Longrightarrow> 
+  Lam\<^sub>d t e = multisubst (map declosure \<Delta>) (Var\<^sub>d x) \<Longrightarrow> 
+    \<exists>\<Delta>' e'. lookup \<Delta> x = Some (Lam\<^sub>c t \<Delta>' e') \<and> 
+      multisubst (map declosure \<Delta>') (Lam\<^sub>d t e') = multisubst (map declosure \<Delta>) (Var\<^sub>d x)"
+proof (induction \<Delta> x arbitrary: \<Gamma> rule: lookup.induct)
+  case (2 c \<Delta>)
+  moreover then obtain \<Gamma>' where "\<Gamma> = tt # \<Gamma>' \<and> (c :\<^sub>c\<^sub>l tt) \<and> (\<Delta> :\<^sub>c\<^sub>l\<^sub>s \<Gamma>')" by auto
+  ultimately show ?case by auto
+qed fastforce+
 
-lemma [dest]: "cs :\<^sub>c\<^sub>l\<^sub>s ts \<Longrightarrow> ts \<turnstile>\<^sub>d e : t' \<Longrightarrow> Lam\<^sub>d t e' = multisubst (map declosure cs) e \<Longrightarrow> 
-  (\<exists>e''. e = Lam\<^sub>d t e'') \<or> (\<exists>x cs' e''. e = Var\<^sub>d x \<and> lookup cs x = Some (Lam\<^sub>c t cs' e'') \<and> 
-    multisubst (map declosure cs') (Lam\<^sub>d t e'') = Lam\<^sub>d t e')"
+lemma multisubst_to_lam [dest]: "\<Delta> :\<^sub>c\<^sub>l\<^sub>s \<Gamma> \<Longrightarrow> \<Gamma> \<turnstile>\<^sub>d e : t' \<Longrightarrow> 
+  Lam\<^sub>d t e' = multisubst (map declosure \<Delta>) e \<Longrightarrow> 
+    (\<exists>e''. e = Lam\<^sub>d t e'') \<or> (\<exists>x \<Delta>' e''. e = Var\<^sub>d x \<and> lookup \<Delta> x = Some (Lam\<^sub>c t \<Delta>' e'') \<and> 
+      multisubst (map declosure \<Delta>') (Lam\<^sub>d t e'') = Lam\<^sub>d t e')"
 proof (induction e)
   case (Lam\<^sub>d t e)
-  moreover then obtain e' where "multisubst (map declosure cs) (Lam\<^sub>d t e) = Lam\<^sub>d t e'" by fastforce
+  moreover then obtain e' where "multisubst (map declosure \<Delta>) (Lam\<^sub>d t e) = Lam\<^sub>d t e'" by fastforce
   ultimately show ?case by simp
 qed auto
 
-lemma [simp]: "lookup cs x = Some c \<Longrightarrow> c :\<^sub>c\<^sub>l t \<Longrightarrow> 
-    multisubst (map declosure cs) (Var\<^sub>d x) = declosure c"
-  by (induction cs x rule: lookup.induct) simp_all
+text \<open>Now we can prove correctness:\<close>
 
-lemma [simp]: "value\<^sub>d (multisubst (map declosure cs) e) \<Longrightarrow> SE\<^sub>c s cs e :\<^sub>c t \<Longrightarrow>
-  \<exists>c. SE\<^sub>c s cs e \<leadsto>\<^sub>c SC\<^sub>c s c \<and> multisubst (map declosure cs) e = declosure c"
-proof (induction e)
-  case (Var\<^sub>d x)
-  then obtain t' ts where "(s :\<^sub>c t' \<rightarrow> t) \<and> (cs :\<^sub>c\<^sub>l\<^sub>s ts) \<and> (lookup ts x = Some t')" by fastforce
-  then obtain c where "lookup cs x = Some c \<and> c :\<^sub>c\<^sub>l t'" by fastforce
-  hence "SE\<^sub>c s cs (Var\<^sub>d x) \<leadsto>\<^sub>c SC\<^sub>c s c \<and> multisubst (map declosure cs) (Var\<^sub>d x) = declosure c" 
-    by fastforce
-  thus ?case by blast
-next
-  case (Const\<^sub>d k)
-  have "SE\<^sub>c s cs (Const\<^sub>d k) \<leadsto>\<^sub>c SC\<^sub>c s (Const\<^sub>c k) \<and> 
-    multisubst (map declosure cs) (Const\<^sub>d k) = declosure (Const\<^sub>c k)" by simp
-  thus ?case by blast
-next
-  case (Lam\<^sub>d tt e)
-  hence "SE\<^sub>c s cs (Lam\<^sub>d tt e) \<leadsto>\<^sub>c SC\<^sub>c s (Lam\<^sub>c tt cs e) \<and> 
-    multisubst (map declosure cs) (Lam\<^sub>d tt e) = declosure (Lam\<^sub>c tt cs e)" by simp
-  thus ?case by blast
-qed simp_all
-
-theorem completec [simp]: "destate\<^sub>c \<Sigma>\<^sub>c \<leadsto>\<^sub>k \<Sigma>\<^sub>s' \<Longrightarrow> \<Sigma>\<^sub>c :\<^sub>c t \<Longrightarrow> 
-    \<exists>\<Sigma>\<^sub>c'. iter (\<leadsto>\<^sub>c) \<Sigma>\<^sub>c \<Sigma>\<^sub>c' \<and> \<Sigma>\<^sub>s' = destate\<^sub>c \<Sigma>\<^sub>c'"
-proof (induction "destate\<^sub>c \<Sigma>\<^sub>c" \<Sigma>\<^sub>s' rule: eval\<^sub>k.induct)
-  case (ev\<^sub>k_const s k)
-  then obtain s' cs e' where S: "s = declosure_stack s' \<and> \<Sigma>\<^sub>c = SE\<^sub>c s' cs e' \<and> 
-    Const\<^sub>d k = multisubst (map declosure cs) e'" by fastforce
+theorem correct\<^sub>c [simp]: "declosure_state \<Sigma>\<^sub>c \<leadsto>\<^sub>k \<Sigma>\<^sub>s' \<Longrightarrow> \<Sigma>\<^sub>c :\<^sub>c t \<Longrightarrow> 
+    \<exists>\<Sigma>\<^sub>c'. iter (\<leadsto>\<^sub>c) \<Sigma>\<^sub>c \<Sigma>\<^sub>c' \<and> \<Sigma>\<^sub>s' = declosure_state \<Sigma>\<^sub>c'"
+proof (induction "declosure_state \<Sigma>\<^sub>c" \<Sigma>\<^sub>s' rule: eval\<^sub>k.induct)
+  case (ev\<^sub>k_const s n)
+  then obtain s' \<Delta> e' where S: "s = declosure_stack s' \<and> \<Sigma>\<^sub>c = SE\<^sub>c s' \<Delta> e' \<and> 
+    Const\<^sub>d n = multisubst (map declosure \<Delta>) e'" by fastforce
   thus ?case
-  proof (cases "e' = Const\<^sub>d k")
+  proof (cases "e' = Const\<^sub>d n")
     case True
-    have "SE\<^sub>c s' cs (Const\<^sub>d k) \<leadsto>\<^sub>c SC\<^sub>c s' (Const\<^sub>c k)" by simp
-    hence "iter (\<leadsto>\<^sub>c) (SE\<^sub>c s' cs (Const\<^sub>d k)) (SC\<^sub>c s' (Const\<^sub>c k))" by (metis iter_refl iter_step)
+    have "SE\<^sub>c s' \<Delta> (Const\<^sub>d n) \<leadsto>\<^sub>c SC\<^sub>c s' (Const\<^sub>c n)" by simp
+    hence "iter (\<leadsto>\<^sub>c) (SE\<^sub>c s' \<Delta> (Const\<^sub>d n)) (SC\<^sub>c s' (Const\<^sub>c n))" by (metis iter_refl iter_step)
     with S True show ?thesis by fastforce
   next
     case False
-    with S obtain x where E: "e' = Var\<^sub>d x \<and> lookup cs x = Some (Const\<^sub>c k)" by fastforce
-    hence "SE\<^sub>c s' cs (Var\<^sub>d x) \<leadsto>\<^sub>c SC\<^sub>c s' (Const\<^sub>c k)" by simp
-    hence X: "iter (\<leadsto>\<^sub>c) (SE\<^sub>c s' cs (Var\<^sub>d x)) (SC\<^sub>c s' (Const\<^sub>c k))" by simp
-    from S have "S\<^sub>k True s (Const\<^sub>d k) = destate\<^sub>c (SC\<^sub>c s' (Const\<^sub>c k))" by simp
+    with S obtain x where E: "e' = Var\<^sub>d x \<and> lookup \<Delta> x = Some (Const\<^sub>c n)" by fastforce
+    hence "SE\<^sub>c s' \<Delta> (Var\<^sub>d x) \<leadsto>\<^sub>c SC\<^sub>c s' (Const\<^sub>c n)" by simp
+    hence X: "iter (\<leadsto>\<^sub>c) (SE\<^sub>c s' \<Delta> (Var\<^sub>d x)) (SC\<^sub>c s' (Const\<^sub>c n))" by simp
+    from S have "S\<^sub>k True s (Const\<^sub>d n) = declosure_state (SC\<^sub>c s' (Const\<^sub>c n))" by simp
     with S E X show ?thesis by blast
   qed
 next
   case (ev\<^sub>k_lam s tt e)
-  then obtain s' cs e' where S: "s = declosure_stack s' \<and> \<Sigma>\<^sub>c = SE\<^sub>c s' cs e' \<and> 
-    Lam\<^sub>d tt e = multisubst (map declosure cs) e'" by fastforce
-  with ev\<^sub>k_lam obtain t' ts where T: "(s' :\<^sub>c t' \<rightarrow> t) \<and> (cs :\<^sub>c\<^sub>l\<^sub>s ts) \<and> 
-    latest_environment s' = Some cs \<and> ts \<turnstile>\<^sub>d e' : t'" by fastforce
+  then obtain s' \<Delta> e' where S: "s = declosure_stack s' \<and> \<Sigma>\<^sub>c = SE\<^sub>c s' \<Delta> e' \<and> 
+    Lam\<^sub>d tt e = multisubst (map declosure \<Delta>) e'" by fastforce
+  with ev\<^sub>k_lam obtain t' \<Gamma> where T: "(s' :\<^sub>c t' \<rightarrow> t) \<and> (\<Delta> :\<^sub>c\<^sub>l\<^sub>s \<Gamma>) \<and> 
+    latest_environment s' = Some \<Delta> \<and> \<Gamma> \<turnstile>\<^sub>d e' : t'" by fastforce
   thus ?case
   proof (cases "\<exists>e''. e' = Lam\<^sub>d tt e''")
     case True
     then obtain e'' where E: "e' = Lam\<^sub>d tt e''" by fastforce
-    have "SE\<^sub>c s' cs (Lam\<^sub>d tt e'') \<leadsto>\<^sub>c SC\<^sub>c s' (Lam\<^sub>c tt cs e'')" by simp
-    hence "iter (\<leadsto>\<^sub>c) (SE\<^sub>c s' cs (Lam\<^sub>d tt e'')) (SC\<^sub>c s' (Lam\<^sub>c tt cs e''))" 
+    have "SE\<^sub>c s' \<Delta> (Lam\<^sub>d tt e'') \<leadsto>\<^sub>c SC\<^sub>c s' (Lam\<^sub>c tt \<Delta> e'')" by simp
+    hence "iter (\<leadsto>\<^sub>c) (SE\<^sub>c s' \<Delta> (Lam\<^sub>d tt e'')) (SC\<^sub>c s' (Lam\<^sub>c tt \<Delta> e''))" 
       by (metis iter_refl iter_step)
     with S E show ?thesis by fastforce
   next
     case False
-    with S T obtain x cs' e'' where E: "e' = Var\<^sub>d x \<and> lookup cs x = Some (Lam\<^sub>c tt cs' e'') \<and> 
-      multisubst (map declosure cs') (Lam\<^sub>d tt e'') = Lam\<^sub>d tt e" by blast
-    hence "SE\<^sub>c s' cs (Var\<^sub>d x) \<leadsto>\<^sub>c SC\<^sub>c s' (Lam\<^sub>c tt cs' e'')" by simp
-    hence X: "iter (\<leadsto>\<^sub>c) (SE\<^sub>c s' cs (Var\<^sub>d x)) (SC\<^sub>c s' (Lam\<^sub>c tt cs' e''))" by simp
-    from S E have "multisubst (map declosure cs) e' = multisubst (map declosure cs') (Lam\<^sub>d tt e'')"
+    with S T obtain x \<Delta>' e'' where E: "e' = Var\<^sub>d x \<and> lookup \<Delta> x = Some (Lam\<^sub>c tt \<Delta>' e'') \<and> 
+      multisubst (map declosure \<Delta>') (Lam\<^sub>d tt e'') = Lam\<^sub>d tt e" by blast
+    hence "SE\<^sub>c s' \<Delta> (Var\<^sub>d x) \<leadsto>\<^sub>c SC\<^sub>c s' (Lam\<^sub>c tt \<Delta>' e'')" by simp
+    hence X: "iter (\<leadsto>\<^sub>c) (SE\<^sub>c s' \<Delta> (Var\<^sub>d x)) (SC\<^sub>c s' (Lam\<^sub>c tt \<Delta>' e''))" by simp
+    from S E have "multisubst (map declosure \<Delta>) e' = multisubst (map declosure \<Delta>') (Lam\<^sub>d tt e'')"
       by metis
-    with S have "S\<^sub>k True s (Lam\<^sub>d tt e) = destate\<^sub>c (SC\<^sub>c s' (Lam\<^sub>c tt cs' e''))" by simp
+    with S have "S\<^sub>k True s (Lam\<^sub>d tt e) = declosure_state (SC\<^sub>c s' (Lam\<^sub>c tt \<Delta>' e''))" by simp
     with S E X show ?thesis by blast
   qed
 next
   case (ev\<^sub>k_app1 s e\<^sub>1 e\<^sub>2)
-  then obtain s' cs e' where S: "s = declosure_stack s' \<and> \<Sigma>\<^sub>c = SE\<^sub>c s' cs e' \<and> 
-    App\<^sub>d e\<^sub>1 e\<^sub>2 = multisubst (map declosure cs) e'" by fastforce
+  then obtain s' \<Delta> e' where S: "s = declosure_stack s' \<and> \<Sigma>\<^sub>c = SE\<^sub>c s' \<Delta> e' \<and> 
+    App\<^sub>d e\<^sub>1 e\<^sub>2 = multisubst (map declosure \<Delta>) e'" by fastforce
   then obtain e\<^sub>1' e\<^sub>2' where E: "e' = App\<^sub>d e\<^sub>1' e\<^sub>2' \<and>
-    e\<^sub>1 = multisubst (map declosure cs) e\<^sub>1' \<and> e\<^sub>2 = multisubst (map declosure cs) e\<^sub>2'" by fastforce                                                  
-  have "SE\<^sub>c s' cs (App\<^sub>d e\<^sub>1' e\<^sub>2') \<leadsto>\<^sub>c SE\<^sub>c (FApp1\<^sub>c cs e\<^sub>2' # s') cs e\<^sub>1'" by simp
-  hence "iter (\<leadsto>\<^sub>c) (SE\<^sub>c s' cs (App\<^sub>d e\<^sub>1' e\<^sub>2')) (SE\<^sub>c (FApp1\<^sub>c cs e\<^sub>2' # s') cs e\<^sub>1')" 
+    e\<^sub>1 = multisubst (map declosure \<Delta>) e\<^sub>1' \<and> e\<^sub>2 = multisubst (map declosure \<Delta>) e\<^sub>2'" by fastforce                                                  
+  have "SE\<^sub>c s' \<Delta> (App\<^sub>d e\<^sub>1' e\<^sub>2') \<leadsto>\<^sub>c SE\<^sub>c (FApp1\<^sub>c \<Delta> e\<^sub>2' # s') \<Delta> e\<^sub>1'" by simp
+  hence "iter (\<leadsto>\<^sub>c) (SE\<^sub>c s' \<Delta> (App\<^sub>d e\<^sub>1' e\<^sub>2')) (SE\<^sub>c (FApp1\<^sub>c \<Delta> e\<^sub>2' # s') \<Delta> e\<^sub>1')" 
     by (metis iter_refl iter_step)
   with S E show ?case by fastforce
 next
   case (ev\<^sub>k_app2 e\<^sub>2 s e\<^sub>1)
   then obtain s\<^sub>c c where S: "FApp1\<^sub>k e\<^sub>2 # s = declosure_stack s\<^sub>c \<and> \<Sigma>\<^sub>c = SC\<^sub>c s\<^sub>c c \<and> e\<^sub>1 = declosure c"
-    by fastforce
-  then obtain cs' e\<^sub>2' s\<^sub>c' where S': "s\<^sub>c = FApp1\<^sub>c cs' e\<^sub>2' # s\<^sub>c' \<and> 
-    e\<^sub>2 = multisubst (map declosure cs') e\<^sub>2' \<and> s = declosure_stack s\<^sub>c'" by fastforce
-  have "SC\<^sub>c (FApp1\<^sub>c cs' e\<^sub>2' # s\<^sub>c') c \<leadsto>\<^sub>c SE\<^sub>c (FApp2\<^sub>c c # s\<^sub>c') cs' e\<^sub>2'" by simp
-  hence "iter (\<leadsto>\<^sub>c) (SC\<^sub>c (FApp1\<^sub>c cs' e\<^sub>2' # s\<^sub>c') c) (SE\<^sub>c (FApp2\<^sub>c c # s\<^sub>c') cs' e\<^sub>2')" 
+    by auto
+  then obtain \<Delta>' e\<^sub>2' s\<^sub>c' where S': "s\<^sub>c = FApp1\<^sub>c \<Delta>' e\<^sub>2' # s\<^sub>c' \<and> 
+    e\<^sub>2 = multisubst (map declosure \<Delta>') e\<^sub>2' \<and> s = declosure_stack s\<^sub>c'" by fastforce
+  have "SC\<^sub>c (FApp1\<^sub>c \<Delta>' e\<^sub>2' # s\<^sub>c') c \<leadsto>\<^sub>c SE\<^sub>c (FApp2\<^sub>c c # s\<^sub>c') \<Delta>' e\<^sub>2'" by simp
+  hence "iter (\<leadsto>\<^sub>c) (SC\<^sub>c (FApp1\<^sub>c \<Delta>' e\<^sub>2' # s\<^sub>c') c) (SE\<^sub>c (FApp2\<^sub>c c # s\<^sub>c') \<Delta>' e\<^sub>2')" 
     by (metis iter_refl iter_step)
   with S S' show ?case by fastforce
 next
   case (ev\<^sub>k_app3 t\<^sub>1 e\<^sub>1 s e\<^sub>2)
   then obtain s\<^sub>c c\<^sub>2 where S: "FApp2\<^sub>k (Lam\<^sub>d t\<^sub>1 e\<^sub>1) # s = declosure_stack s\<^sub>c \<and> \<Sigma>\<^sub>c = SC\<^sub>c s\<^sub>c c\<^sub>2 \<and> 
-    e\<^sub>2 = declosure c\<^sub>2" by fastforce
+    e\<^sub>2 = declosure c\<^sub>2" by auto
   then obtain c s\<^sub>c' where S': "s\<^sub>c = FApp2\<^sub>c c # s\<^sub>c' \<and> Lam\<^sub>d t\<^sub>1 e\<^sub>1 = declosure c \<and> 
     s = declosure_stack s\<^sub>c'" by fastforce
-  from ev\<^sub>k_app3 S S' obtain t' t\<^sub>2 cs where T: "(c :\<^sub>c\<^sub>l Arrow t' t\<^sub>2) \<and> (s\<^sub>c' :\<^sub>c t\<^sub>2 \<rightarrow> t) \<and> 
-    latest_environment s\<^sub>c' = Some cs \<and> c\<^sub>2 :\<^sub>c\<^sub>l t'" by fastforce
-  with S' obtain cs' e\<^sub>1' where C: "c = Lam\<^sub>c t\<^sub>1 cs' e\<^sub>1' \<and> 
-    multisubst (map declosure cs') (Lam\<^sub>d t\<^sub>1 e\<^sub>1') = Lam\<^sub>d t\<^sub>1 e\<^sub>1 \<and> ([t\<^sub>1] \<turnstile>\<^sub>d e\<^sub>1 : t\<^sub>2) \<and> t' = t\<^sub>1 \<and>
-    (\<forall>e\<^sub>2. ([] \<turnstile>\<^sub>d e\<^sub>2 : t\<^sub>1) \<longrightarrow> multisubst (map declosure cs') (subst\<^sub>d 0 e\<^sub>2 e\<^sub>1') = subst\<^sub>d 0 e\<^sub>2 e\<^sub>1)" 
-      by (metis lam_to_declosure)
-  with T S have "subst\<^sub>d 0 e\<^sub>2 e\<^sub>1 = multisubst (map declosure cs') (subst\<^sub>d 0 (declosure c\<^sub>2) e\<^sub>1')" 
+  from ev\<^sub>k_app3 S S' obtain t' t\<^sub>2 \<Delta> where T: "(c :\<^sub>c\<^sub>l Arrow t' t\<^sub>2) \<and> (s\<^sub>c' :\<^sub>c t\<^sub>2 \<rightarrow> t) \<and> 
+    latest_environment s\<^sub>c' = Some \<Delta> \<and> c\<^sub>2 :\<^sub>c\<^sub>l t'" by fastforce
+  with S' obtain \<Delta>' e\<^sub>1' where C: "c = Lam\<^sub>c t\<^sub>1 \<Delta>' e\<^sub>1' \<and> 
+    multisubst (map declosure \<Delta>') (Lam\<^sub>d t\<^sub>1 e\<^sub>1') = Lam\<^sub>d t\<^sub>1 e\<^sub>1 \<and> ([t\<^sub>1] \<turnstile>\<^sub>d e\<^sub>1 : t\<^sub>2) \<and> t' = t\<^sub>1 \<and>
+    (\<forall>e\<^sub>2. ([] \<turnstile>\<^sub>d e\<^sub>2 : t\<^sub>1) \<longrightarrow> multisubst (map declosure \<Delta>') (subst\<^sub>d 0 e\<^sub>2 e\<^sub>1') = subst\<^sub>d 0 e\<^sub>2 e\<^sub>1)" 
+      by (metis declose_to_lam)
+  with T S have "subst\<^sub>d 0 e\<^sub>2 e\<^sub>1 = multisubst (map declosure \<Delta>') (subst\<^sub>d 0 (declosure c\<^sub>2) e\<^sub>1')" 
     by simp
   with S S' have X: "S\<^sub>k False (FReturn\<^sub>k # s) (subst\<^sub>d 0 e\<^sub>2 e\<^sub>1) = 
-    destate\<^sub>c (SE\<^sub>c (FReturn\<^sub>c (c\<^sub>2 # cs') # s\<^sub>c') (c\<^sub>2 # cs') e\<^sub>1')" by simp
-  have "SC\<^sub>c (FApp2\<^sub>c (Lam\<^sub>c t\<^sub>1 cs' e\<^sub>1') # s\<^sub>c') c\<^sub>2 \<leadsto>\<^sub>c SE\<^sub>c (FReturn\<^sub>c (c\<^sub>2 # cs') # s\<^sub>c') (c\<^sub>2 # cs') e\<^sub>1'"
+    declosure_state (SE\<^sub>c (FReturn\<^sub>c (c\<^sub>2 # \<Delta>') # s\<^sub>c') (c\<^sub>2 # \<Delta>') e\<^sub>1')" by simp
+  have "SC\<^sub>c (FApp2\<^sub>c (Lam\<^sub>c t\<^sub>1 \<Delta>' e\<^sub>1') # s\<^sub>c') c\<^sub>2 \<leadsto>\<^sub>c SE\<^sub>c (FReturn\<^sub>c (c\<^sub>2 # \<Delta>') # s\<^sub>c') (c\<^sub>2 # \<Delta>') e\<^sub>1'"
     by simp
   with S S' C X show ?case by (metis iter_step iter_refl)
 next
   case (ev\<^sub>k_ret s e)
   then obtain s\<^sub>c c where S: "FReturn\<^sub>k # s = declosure_stack s\<^sub>c \<and> \<Sigma>\<^sub>c = SC\<^sub>c s\<^sub>c c \<and> e = declosure c" 
     by fastforce
-  then obtain cs s\<^sub>c' where S': "s\<^sub>c = FReturn\<^sub>c cs # s\<^sub>c'" by fastforce
-  have "SC\<^sub>c (FReturn\<^sub>c cs # s\<^sub>c') c \<leadsto>\<^sub>c SC\<^sub>c s\<^sub>c' c" by simp
-  hence "iter (\<leadsto>\<^sub>c) (SC\<^sub>c (FReturn\<^sub>c cs # s\<^sub>c') c) (SC\<^sub>c s\<^sub>c' c)" by (metis iter_refl iter_step)
+  then obtain \<Delta> s\<^sub>c' where S': "s\<^sub>c = FReturn\<^sub>c \<Delta> # s\<^sub>c'" by fastforce
+  have "SC\<^sub>c (FReturn\<^sub>c \<Delta> # s\<^sub>c') c \<leadsto>\<^sub>c SC\<^sub>c s\<^sub>c' c" by simp
+  hence "iter (\<leadsto>\<^sub>c) (SC\<^sub>c (FReturn\<^sub>c \<Delta> # s\<^sub>c') c) (SC\<^sub>c s\<^sub>c' c)" by (metis iter_refl iter_step)
   with S S' show ?case by fastforce
 qed
 
-lemma [simp]: "iter (\<leadsto>\<^sub>k) (destate\<^sub>c \<Sigma>\<^sub>c) \<Sigma>\<^sub>s' \<Longrightarrow> \<Sigma>\<^sub>c :\<^sub>c t \<Longrightarrow> 
-  \<exists>\<Sigma>\<^sub>c'. iter (\<leadsto>\<^sub>c) \<Sigma>\<^sub>c \<Sigma>\<^sub>c' \<and> \<Sigma>\<^sub>s' = destate\<^sub>c \<Sigma>\<^sub>c'"
-proof (induction "destate\<^sub>c \<Sigma>\<^sub>c" \<Sigma>\<^sub>s' arbitrary: \<Sigma>\<^sub>c rule: iter.induct)
+lemma correct\<^sub>c_iter [simp]: "iter (\<leadsto>\<^sub>k) (declosure_state \<Sigma>\<^sub>c) \<Sigma>\<^sub>s' \<Longrightarrow> \<Sigma>\<^sub>c :\<^sub>c t \<Longrightarrow> 
+  \<exists>\<Sigma>\<^sub>c'. iter (\<leadsto>\<^sub>c) \<Sigma>\<^sub>c \<Sigma>\<^sub>c' \<and> \<Sigma>\<^sub>s' = declosure_state \<Sigma>\<^sub>c'"
+proof (induction "declosure_state \<Sigma>\<^sub>c" \<Sigma>\<^sub>s' arbitrary: \<Sigma>\<^sub>c rule: iter.induct)
   case (iter_step \<Sigma>\<^sub>s' \<Sigma>\<^sub>s'')
-  moreover then obtain \<Sigma>\<^sub>c' where X: "iter (\<leadsto>\<^sub>c) \<Sigma>\<^sub>c \<Sigma>\<^sub>c' \<and> \<Sigma>\<^sub>s' = destate\<^sub>c \<Sigma>\<^sub>c'" by fastforce
+  moreover then obtain \<Sigma>\<^sub>c' where X: "iter (\<leadsto>\<^sub>c) \<Sigma>\<^sub>c \<Sigma>\<^sub>c' \<and> \<Sigma>\<^sub>s' = declosure_state \<Sigma>\<^sub>c'" by fastforce
   moreover with iter_step have "\<Sigma>\<^sub>c' :\<^sub>c t" by fastforce
-  ultimately obtain \<Sigma>\<^sub>c'' where "iter (\<leadsto>\<^sub>c) \<Sigma>\<^sub>c' \<Sigma>\<^sub>c'' \<and> \<Sigma>\<^sub>s'' = destate\<^sub>c \<Sigma>\<^sub>c''" by fastforce
-  with X have "iter (\<leadsto>\<^sub>c) \<Sigma>\<^sub>c \<Sigma>\<^sub>c'' \<and> \<Sigma>\<^sub>s'' = destate\<^sub>c \<Sigma>\<^sub>c''" by (metis iter_append)
+  ultimately obtain \<Sigma>\<^sub>c'' where "iter (\<leadsto>\<^sub>c) \<Sigma>\<^sub>c' \<Sigma>\<^sub>c'' \<and> \<Sigma>\<^sub>s'' = declosure_state \<Sigma>\<^sub>c''" by fastforce
+  with X have "iter (\<leadsto>\<^sub>c) \<Sigma>\<^sub>c \<Sigma>\<^sub>c'' \<and> \<Sigma>\<^sub>s'' = declosure_state \<Sigma>\<^sub>c''" by (metis iter_append)
   thus ?case by fastforce
 qed force+
 
-lemma [simp]: "value\<^sub>d (multisubst (map declosure cs) e) \<Longrightarrow> \<exists>c. SE\<^sub>c s cs e \<leadsto>\<^sub>c SC\<^sub>c s c" 
-proof (induction e)
-  case (Var\<^sub>d x)
-  then obtain c where "lookup cs x = Some c" by (induction cs x rule: lookup.induct) simp_all
-  hence "SE\<^sub>c s cs (Var\<^sub>d x) \<leadsto>\<^sub>c SC\<^sub>c s c" by simp
-  thus ?case by fastforce
-next
-  case (Const\<^sub>d k)
-  have "SE\<^sub>c s cs (Const\<^sub>d k) \<leadsto>\<^sub>c SC\<^sub>c s (Const\<^sub>c k)" by simp
-  thus ?case by fastforce
-next
-  case (Lam\<^sub>d t e)
-  have "SE\<^sub>c s cs (Lam\<^sub>d t e) \<leadsto>\<^sub>c SC\<^sub>c s (Lam\<^sub>c t cs e)" by simp
-  thus ?case by fastforce
-qed simp_all
-
-lemma [simp]: "\<Sigma>\<^sub>c :\<^sub>c t \<Longrightarrow> iter (\<leadsto>\<^sub>k) (destate\<^sub>c \<Sigma>\<^sub>c) (S\<^sub>k True [] v) \<Longrightarrow> 
+lemma correct\<^sub>c_full_eval [simp]: "\<Sigma>\<^sub>c :\<^sub>c t \<Longrightarrow> iter (\<leadsto>\<^sub>k) (declosure_state \<Sigma>\<^sub>c) (S\<^sub>k True [] v) \<Longrightarrow> 
   \<exists>c. iter (\<leadsto>\<^sub>c) \<Sigma>\<^sub>c (SC\<^sub>c [] c) \<and> declosure c = v"
 proof -
-  assume TC: "\<Sigma>\<^sub>c :\<^sub>c t" and "iter (\<leadsto>\<^sub>k) (destate\<^sub>c \<Sigma>\<^sub>c) (S\<^sub>k True [] v)"
-  then obtain \<Sigma>\<^sub>c' where E: "iter (\<leadsto>\<^sub>c) \<Sigma>\<^sub>c \<Sigma>\<^sub>c' \<and> S\<^sub>k True [] v = destate\<^sub>c \<Sigma>\<^sub>c'" by fastforce
+  assume TC: "\<Sigma>\<^sub>c :\<^sub>c t" and "iter (\<leadsto>\<^sub>k) (declosure_state \<Sigma>\<^sub>c) (S\<^sub>k True [] v)"
+  then obtain \<Sigma>\<^sub>c' where E: "iter (\<leadsto>\<^sub>c) \<Sigma>\<^sub>c \<Sigma>\<^sub>c' \<and> S\<^sub>k True [] v = declosure_state \<Sigma>\<^sub>c'" by fastforce
   then obtain s' c where "[] = declosure_stack s' \<and> \<Sigma>\<^sub>c' = SC\<^sub>c s' c \<and> v = declosure c" by fastforce
-  moreover hence "s' = []" by simp
-  ultimately have S: "(\<exists>cs e. \<Sigma>\<^sub>c' = SE\<^sub>c [] cs e \<and> v = multisubst (map declosure cs) e) \<or> 
-    (\<exists>c. \<Sigma>\<^sub>c' = SC\<^sub>c [] c \<and> v = declosure c)" by simp
+  hence "(\<exists>\<Delta> e. \<Sigma>\<^sub>c' = SE\<^sub>c [] \<Delta> e \<and> v = multisubst (map declosure \<Delta>) e) \<or> 
+    (\<exists>c. \<Sigma>\<^sub>c' = SC\<^sub>c [] c \<and> v = declosure c)" by auto
   with E show ?thesis by fastforce
 qed
 
